Nemonuri/TransitionSystemLike/ProgramGraph/Interleaving.lean
@@ -17,29 +17,165 @@ namespace Nemonuri.ProgramGraph
 
 open HasHUnion
 
-namespace Eval
+namespace EvalLike
 
-universe uvar_l uval_l uvar_r uval_r
+universe uvar_l uval_l uec uvar_r uval_r uec_r
+
+structure IsInterleaving
+  (VarL1 VarL2: Type uvar_l) (ValL1 ValL2: Type uval_l) (EC1 EC2: Type uec) [EvalLike EC1 VarL1 ValL1] [EvalLike EC2 VarL2 ValL2]
+  (VarR: Type uvar_r) (ValR: Type uval_r) [HasHUnion VarL1 VarL2 VarR] [HasHUnion ValL1 ValL2 ValR]
+  (toEval: EC1 → EC2 → (HUnionElemAt VarL1 VarL2 VarR) → (HUnionElemAt ValL1 ValL2 ValR)) : Prop where
+  diff_fst (x: HDiffElemAt VarL1 VarL2 VarR .fst) (ec1: EC1) (ec2: EC2) :
+    .ofEmbedElem (EmbedElemAt.mapAt VarL1 VarL2 ValL1 ValL2 .fst (ec1: Eval VarL1 ValL1) x.toEmbedElem) = toEval ec1 ec2 (.ofEmbedElem x.toEmbedElem)
+  diff_snd (x: HDiffElemAt VarL1 VarL2 VarR .snd) (ec1: EC1) (ec2: EC2) :
+    .ofEmbedElem (EmbedElemAt.mapAt VarL1 VarL2 ValL1 ValL2 .snd (ec2: Eval VarL2 ValL2) x.toEmbedElem) = toEval ec1 ec2 (.ofEmbedElem x.toEmbedElem)
+  inter (x: HInterElemAt VarL1 VarL2 VarR) (ec1: EC1) (ec2: EC2) :
+    let rhs := toEval ec1 ec2 (x.toUnion)
+    (.ofEmbedElem (EmbedElemAt.mapAt VarL1 VarL2 ValL1 ValL2 .fst (ec1: Eval VarL1 ValL1) (x.toEmbedElemAt .fst)) = rhs) ∨
+    (.ofEmbedElem (EmbedElemAt.mapAt VarL1 VarL2 ValL1 ValL2 .snd (ec2: Eval VarL2 ValL2) (x.toEmbedElemAt .snd)) = rhs)
+
 
 structure Interleaving
-  {VarL1 VarL2: Type uvar_l} {ValL1 ValL2: Type uval_l}
-  (ec1 : Eval VarL1 ValL1) (ec2: Eval VarL2 ValL2) (VarR: Type uvar_r) (ValR: Type uval_r) where
-  var: Bundle VarL1 VarL2 VarR
-  val: Bundle ValL1 ValL2 ValR
-  sel: letI := var.hasHUnion; HInterElemAt VarL1 VarL2 VarR → Label
+  (VarL1 VarL2: Type uvar_l) (ValL1 ValL2: Type uval_l) (EC1 EC2: Type uec) [EvalLike EC1 VarL1 ValL1] [EvalLike EC2 VarL2 ValL2]
+  (VarR: Type uvar_r) (ValR: Type uval_r) [HasHUnion VarL1 VarL2 VarR] [HasHUnion ValL1 ValL2 ValR] where
+  toEval (ec1: EC1) (ec2: EC2) : (HUnionElemAt VarL1 VarL2 VarR) → (HUnionElemAt ValL1 ValL2 ValR)
+  valid: IsInterleaving VarL1 VarL2 ValL1 ValL2 EC1 EC2 VarR ValR toEval
+
 
 namespace Interleaving
 
-variable {VarL1 VarL2: Type uvar_l} {ValL1 ValL2: Type uval_l}
-         {ec1 : Eval VarL1 ValL1} {ec2: Eval VarL2 ValL2} {VarR: Type uvar_r} {ValR: Type uval_r}
+inductive OfEvalCarriers
+  (VarL1 VarL2: Type uvar_l) (ValL1 ValL2: Type uval_l) (EC1 EC2: Type uec) [EvalLike EC1 VarL1 ValL1] [EvalLike EC2 VarL2 ValL2]
+  (VarR: Type uvar_r) (ValR: Type uval_r) [HasHUnion VarL1 VarL2 VarR] [HasHUnion ValL1 ValL2 ValR]
+  : EC1 → EC2 → Type _ where
+  | mk (il: Interleaving VarL1 VarL2 ValL1 ValL2 EC1 EC2 VarR ValR) (ec1: EC1) (ec2: EC2)
+    : OfEvalCarriers VarL1 VarL2 ValL1 ValL2 EC1 EC2 VarR ValR ec1 ec2
 
-set_option trace.Meta.synthInstance true in
-def eval (il: Interleaving ec1 ec2 VarR ValR) : (letI := il.var; HUnionElemAt VarL1 VarL2 VarR) → ValR :=
-  letI := il.var.hasHUnion; letI := il.var.memDecidable
-  letI := il.val.hasHUnion; letI := il.val.memDecidable
+namespace OfEvalCarriers
+
+variable {VarL1 VarL2: Type uvar_l} {ValL1 ValL2: Type uval_l} {EC1 EC2: Type uec} [EvalLike EC1 VarL1 ValL1] [EvalLike EC2 VarL2 ValL2]
+         {VarR: Type uvar_r} {ValR: Type uval_r} [HasHUnion VarL1 VarL2 VarR] [HasHUnion ValL1 ValL2 ValR]
+         {ec1: EC1} {ec2: EC2}
+
+def eval (il: OfEvalCarriers VarL1 VarL2 ValL1 ValL2 EC1 EC2 VarR ValR ec1 ec2) : (HUnionElemAt VarL1 VarL2 VarR) → (HUnionElemAt ValL1 ValL2 ValR) :=
+  il.casesOn (fun il ec1 ec2 => il.toEval ec1 ec2)
+
+/-
+theorem eval_injective : Function.Injective (@eval VarL1 VarL2 ValL1 ValL2 EC1 EC2 _ _ VarR ValR _ _ ec1 ec2) := by
+  rintro ⟨il1, ec1_1, ec2_1⟩ ⟨il2, ec1_2, ec2_2⟩ lm1
+  obtain ⟨te1, lm_v1⟩ := il1
+  obtain ⟨te2, lm_v2⟩ := il2
+  simp
+  dsimp [eval] at lm1
+  simp only [funext_iff] at lm1 ⊢
+  intro ec1_2 ec2_2 x
+  specialize lm1 x
+  obtain ⟨lm_v1_1, lm_v1_2, lm_v1_3⟩ := lm_v1
+  obtain ⟨lm_v2_1, lm_v2_2, lm_v2_3⟩ := lm_v2
+  let decMemVar := DecidableEmbedRange.ofClassicalAt VarL1 VarL2
+  let decMemVal := DecidableEmbedRange.ofClassicalAt ValL1 ValL2
+  cases x using HUnionElemAt.recDiffInter <;> rename_i x
+  · specialize lm_v1_1 x ec1_2 ec2_2
+    specialize lm_v2_1 x ec1_2 ec2_2
+    exact lm_v1_1.symm.trans lm_v2_1
+  · specialize lm_v1_2 x ec1_2 ec2_2
+    specialize lm_v2_2 x ec1_2 ec2_2
+    exact lm_v1_2.symm.trans lm_v2_2
+  · clear lm_v1_1 lm_v2_1 lm_v1_2 lm_v2_2
+    specialize lm_v1_3 x
+    specialize lm_v2_3 x
+    dsimp [HUnionElemAt.ofEmbedElem, HInterElemAt.toEmbedElemAt, HInterElemAt.liftAt, EmbedElemAt.mapAt, EmbedElemAt.bindAt, EmbedElemAt.pureAt, EmbedElemAt.liftAt] at lm_v1_3 lm_v2_3
+    simp only [embedAt_liftAt_eq, Subtype.ext_iff] at lm_v1_3 lm_v2_3
+    simp only [Subtype.ext_iff] at lm1 ⊢
+-/
+    --specialize lm_v1_3 ec1_2 ec2_2
+    --specialize lm_v2_3 ec1_2 ec2_2
+/-
+    rcases lm_v1_3 with lm_v1_3 | lm_v1_3
+    <;> rcases lm_v2_3 with lm_v2_3 | lm_v2_3
+    · exact lm_v1_3.symm.trans lm_v2_3
+    ·
+-/
+/-
+      obtain ⟨x, lm2⟩ := x
+      simp at lm_v1_3 lm_v2_3
+      revert lm2
+      simp [hinterSetUnivAt_mem_iff, LeftTypeAt]
+      intro xl1 lm1 xl2 lm2 lm3 lm4 lm5
+      have lm4_1 := lm4
+      conv at lm4_1 => lhs; simp [← lm1, embedAt_liftAt_eq]
+      have lm5_1 := lm5
+      conv at lm5_1 => lhs; simp [← lm2, embedAt_liftAt_eq]
+      rw [← lm4_1, ← lm5_1]
+      have lm1_1 := @embedAt_liftAt_eq VarL1 VarL2 VarR _ .fst xl1
+      --have lm1_1 := congrArg (liftAt _ _ _ _) lm1
+-/
+    --have lm2 := lm_v1_3 ec1 ec2
+    --have lm3 := lm_v2_3 ec1 ec2
+/-
+    specialize lm_v1_3 x ec1_2 ec2
+    specialize lm_v2_3 x ec1 ec2_2
+    dsimp at lm_v1_3 lm_v2_3
+    rcases lm_v1_3 with lm_v1_3 | lm_v1_3
+    · rcases lm_v2_3 with lm_v2_3 | lm_v2_3
+-/
+/-
+    · rewrite [lm_v1_3] at lm_v2_3
+      rcases lm_v2_3 with lm_v2_3 | lm_v2_3
+      · subst rhs1
+        subst rhs2
+        exact lm_v2_3
+      · subst rhs1
+        subst rhs2
+        rewrite [Subtype.ext_iff] at lm_v1_3 lm_v2_3 lm1 ⊢
+        dsimp [HUnionElemAt.ofEmbedElem, HInterElemAt.toEmbedElemAt, HInterElemAt.liftAt, EmbedElemAt.mapAt, EmbedElemAt.bindAt, EmbedElemAt.pureAt, EmbedElemAt.liftAt] at lm_v1_3 lm_v2_3
+        simp only [embedAt_liftAt_eq] at lm_v1_3 lm_v2_3
+-/
+        --rw [← lm_v1_3, ← lm_v2_3]
+    --specialize lm_v2_1 x ec1_2 ec2_2
+
+  --revert ec1 ec2
+
+
+
+
+end OfEvalCarriers
+
+
+
+/-
+def eval (il: Interleaving ec1 ec2 VarR ValR) : (letI := var.hasHUnion; HUnionElemAt VarL1 VarL2 VarR) → ValR :=
+  letI := var.hasHUnion; letI := var.memDecidable
+  letI := val.hasHUnion; letI := val.memDecidable
   hunionMapAt VarL1 VarL2 VarR ValL1 ValL2 ValR (ec1: VarL1 → ValL1) (ec2: VarL2 → ValL2) il.sel
 
+open DecidableEmbedRange in
+theorem eval_injective : Function.Injective (@eval VarL1 VarL2 ValL1 ValL2 ec1 ec2 VarR ValR _ _) := by
+  rintro ⟨sel1⟩ ⟨sel2⟩ lm1
+  dsimp [eval] at lm1
+  simp
+  simp only [funext_iff] at lm1 ⊢
+  rintro ⟨x, lm2⟩
+  let var_hu := var.hasHUnion
+  let var_md := var.memDecidable
+  specialize lm1 ⟨x, hunionSetUnivAt_mem_of_hinterSetUnivAt_mem lm2⟩
+  obtain ⟨lm3, lm4⟩ := hinterSetUnivAt_mem_iff_isInEmbedRangeAt.mp lm2
+  simp [hunionMapAt, lm3, lm4] at lm1
+  cases lm5: sel1 ⟨x, lm2⟩ <;> cases lm6: sel2 ⟨x, lm2⟩
+  <;> try rfl
+  · simp [lm5, lm6] at lm1
+    revert lm3 lm4
+    simp [isInEmbedRangeAt_eq_true_iff, EmbedRangeAt, LeftTypeAt]
+    intro var_l1 lm3 var_l2 lm4 lm7
+    --have lm8 := @embedAt_injective VarL1 VarL2 VarR _ .fst
+    --have lm9 := @embedAt_injective VarL1 VarL2 VarR _ .snd
+    conv at lm7 =>
+      conv => lhs; simp only [← lm3, embedAt_liftAt_eq]
+      conv => rhs; simp only [← lm4, embedAt_liftAt_eq]
+    skip
 
+    --simp [isInEmbedRangeAt_eq_true_iff, EmbedRangeAt] at lm3 lm4
+-/
 
 
 
@@ -47,7 +183,7 @@ end Interleaving
 
 
 
-end Eval
+end EvalLike
 
 
 --structure Interleaving
